Added PerfExpr type and some axioms; refactored proof and tagging
...to work with PerfExpr

ironfleet/src/Dafny/Distributed/Common/Framework/Performance.s.dfy
@@ -6,6 +6,7 @@ include "../Collections/Seqs.i.dfy"
 module Performance_s {
   import opened Collections__Seqs_i
 
+  /*
   datatype PerformanceReport = PerfVoid | PerfZero | PerformanceReport(instructions: int, pktsDelivered: int)
   type PerfReport = PerformanceReport
 
@@ -23,9 +24,26 @@ module Performance_s {
   function {:axiom} PerfAdd(prs:multiset<PerformanceReport>) : PerformanceReport
     ensures PerfVoid() in prs ==> PerfAdd(prs) == PerfVoid()
     ensures PerfAdd(prs) == PerfAdd(prs[PerfZero() := 0])
+    ensures forall s:multiset<PerformanceReport> :: var p := PerfAdd(s); p in prs ==> PerfAdd(prs) == PerfAdd(prs[p := prs[p] - 1])
 
   function {:axiom} PerfAdd2(pr1:PerformanceReport, pr2:PerformanceReport) : PerformanceReport
     ensures PerfAdd2(pr1, pr2) == PerfAdd(multiset{pr1, pr2})
     ensures pr1 == PerfVoid ==> PerfAdd2(pr1, pr2) == PerfVoid()
     ensures pr2 == PerfVoid ==> PerfAdd2(pr1, pr2) == PerfVoid()
+    */
+
+  datatype PerfExpr = PerfVoid | PerfZero | PerfAdd(prs:multiset<PerfExpr>) | PerfMax(prs:multiset<PerfExpr>)
+  type PerformanceReport = PerfExpr
+  type PerfReport = PerfExpr
+
+  function PerfAdd2(p1:PerfExpr, p2:PerfExpr) : PerfExpr
+  {
+    PerfAdd(multiset{p1, p2})
+  }
+
+  predicate {:axiom} PerfEq(p1:PerfExpr, p2:PerfExpr)
+    ensures p1 == p2 ==> PerfEq(p1, p2)
+    ensures p1.PerfMax? && p1.prs == multiset{p2} ==> PerfEq(p1, p2)
+    ensures p1.PerfMax? && p1.prs == multiset{} && p2 == PerfZero() ==> PerfEq(p1, p2)
+    ensures p1.PerfAdd? && PerfVoid in p1.prs && p2 == PerfZero
 }
